semantics/primTypesScript.sml
@@ -32,7 +32,7 @@ Definition prim_sem_env_def:
   prim_sem_env (ffi:'ffi ffi_state) =
   add_to_sem_env
   (<|clock := 0; ffi := ffi; refs := []; next_type_stamp := 0;
-     next_exn_stamp := 0; eval_state := NONE; ptr_eq_oracle := (K F);
+     next_exn_stamp := 0; eval_state := NONE; ptr_eq_oracle := (K (K F));
    |>,
    <|v := nsEmpty; c := nsEmpty|>) prim_types_program
 End
