semantics/proofs/evaluatePropsScript.sml
@@ -763,8 +763,9 @@ Theorem evaluate_App_PtrEq:
       (case do_eq v1 v2 of
          Eq_type_error => (st', Rerr (Rabort Rtype_error))
        | Eq_val b =>
-           (st' with ptr_eq_oracle := (λn. st'.ptr_eq_oracle (n + 1)),
-            Rval [Boolv (b ∧ st'.ptr_eq_oracle 0)]))
+           (st' with ptr_eq_oracle :=
+              (0 =+ shift_seq 1 (st'.ptr_eq_oracle 0)) st'.ptr_eq_oracle,
+            Rval [Boolv (b ∧ st'.ptr_eq_oracle 0 0)]))
   | _ => (st', Rerr (Rabort Rtype_error))
 Proof
   rw [evaluate_def, fix_clock_evaluate]
@@ -775,7 +776,8 @@ Theorem ptr_eq_sound:
   evaluate st env [App PtrEq es] = (st', Rval [v]) ⇒
   ∃st1 v1 v2 b.
     evaluate st env (REVERSE es) = (st1, Rval [v2; v1]) ∧
-    st' = st1 with ptr_eq_oracle := (λn. st1.ptr_eq_oracle (n + 1)) ∧
+    st' = st1 with ptr_eq_oracle :=
+            (0 =+ shift_seq 1 (st1.ptr_eq_oracle 0)) st1.ptr_eq_oracle ∧
     v = Boolv b ∧
     (b ⇒ do_eq v1 v2 = Eq_val T)
 Proof
